src/Unify.v
@@ -976,12 +976,3 @@ Fixpoint id_in_subst (i : id) (s : substitution) : option ty :=
     | nil => None
     | (i', tau)::s' => if eq_id_dec i i' then Some tau else id_in_subst i s'
   end.
-
-Lemma apply_subst_app1 : forall (s1 s2 : substitution) (st : id),
- id_in_subst st s1 = None -> apply_subst (s1 ++ s2) (var st) = apply_subst s2 (var st).
-Admitted.
-
-Lemma apply_subst_app2 : forall (s1 s2 : substitution) (st : id),
- id_in_subst st s2 = None -> apply_subst (s1 ++ s2) (var st) = apply_subst s1 (var st).
-Admitted.
-
